txn-data-consistency/Prot_2PC_2PL.thy
@@ -8,175 +8,201 @@ subsection \<open>2PC Event system\<close>
 
 subsubsection \<open>State\<close>
 
-datatype status_rm = working | prepared | read_lock | write_lock | no_lock | notokay | committed | aborted
+datatype status_km = working | prepared | read_lock | write_lock | no_lock | notokay | committed | aborted
 datatype status_tm = tm_init | tm_prepared | tm_committed | tm_aborted
 
+\<comment>\<open>Transaction Manager (TM)\<close>
 record tm_state =
   tm_status :: status_tm
   tm_sn :: nat
-  (*tm_view :: view*)
+  (*tm_view :: view -- We used the global_view (seeing everything)*)
 
-record 'v rm_state =
-  rm_db :: "'v version list"
-  rm_fingerpr :: "txid0 \<Rightarrow> 'v key_fp"
-  rm_status :: "txid0 \<Rightarrow> status_rm"
+\<comment>\<open>Key Manager (KM)\<close>
+record 'v km_state =
+  km_vl :: "'v version list"
+  km_key_fp :: "txid0 \<Rightarrow> 'v key_fp"
+  km_status :: "txid0 \<Rightarrow> status_km"
 
+\<comment>\<open>System Global State: TM and KMs\<close>
 record 'v global_state =
   tm :: "cl_id \<Rightarrow> tm_state"
-  rms :: "key \<Rightarrow> 'v rm_state"
+  kms :: "key \<Rightarrow> 'v km_state"
 
 
 subsubsection \<open>Events\<close>
 
-datatype 'v rm_ev = Write2 txid0 'v | Read2 txid0 'v | Prepare txid0 | RLock txid0 | WLock txid0 |
+datatype 'v km_ev = Write2 txid0 'v | Read2 txid0 'v | Prepare txid0 | RLock txid0 | WLock txid0 |
                     NoLock txid0 | NOK txid0 | Commit txid0 | Abort txid0
 datatype tm_ev = User_Commit | TM_Commit | TM_Abort | TM_ReadyC | TM_ReadyA | TM_Skip
-datatype 'v ev = RM_ev key "'v rm_ev" | TM_ev cl_id tm_ev
+datatype 'v ev = KM_ev key "'v km_ev" | TM_ev cl_id tm_ev
 
 definition other_instances_unchanged where
-  "other_instances_unchanged t k rmss rmss' \<equiv> (\<forall>t'. t' \<noteq> t \<longrightarrow>
-     rm_fingerpr (rmss' k) t' = rm_fingerpr (rmss k) t' \<and>
-     rm_status (rmss' k) t' = rm_status (rmss k) t')"
+  "other_instances_unchanged t k kmss kmss' \<equiv> (\<forall>t'. t' \<noteq> t \<longrightarrow>
+     km_key_fp (kmss' k) t' = km_key_fp (kmss k) t' \<and>
+     km_status (kmss' k) t' = km_status (kmss k) t')"
 
-definition other_rms_unchanged where
-  "other_rms_unchanged k rmss rmss' \<equiv> (\<forall>k'. k' \<noteq> k \<longrightarrow> rmss' k' = rmss k')"
+definition other_kms_unchanged where
+  "other_kms_unchanged k kmss kmss' \<equiv> (\<forall>k'. k' \<noteq> k \<longrightarrow> kmss' k' = kmss k')"
 
-abbreviation tm_other_rms_unchanged where
-  "tm_other_rms_unchanged k s s' t \<equiv> tm s' = tm s \<and>
-    other_rms_unchanged k (rms s) (rms s') \<and> other_instances_unchanged t k (rms s) (rms s')"
+abbreviation tm_other_kms_unchanged where
+  "tm_other_kms_unchanged k s s' t \<equiv> tm s' = tm s \<and>
+    other_kms_unchanged k (kms s) (kms s') \<and> other_instances_unchanged t k (kms s) (kms s')"
 
-abbreviation rm_status_trans where
-  "rm_status_trans s k s' t from_stat to_stat \<equiv>
-      rm_status (rms s k) t = from_stat
-    \<and> rm_db (rms s' k) = rm_db (rms s k)
-    \<and> rm_fingerpr (rms s' k) = rm_fingerpr (rms s k)
-    \<and> rm_status (rms s' k) t = to_stat
-    \<and> tm_other_rms_unchanged k s s' t"
+abbreviation km_status_trans where
+  "km_status_trans s k s' t from_stat to_stat \<equiv>
+      km_status (kms s k) t = from_stat
+    \<and> km_vl (kms s' k) = km_vl (kms s k)
+    \<and> km_key_fp (kms s' k) = km_key_fp (kms s k)
+    \<and> km_status (kms s' k) t = to_stat
+    \<and> tm_other_kms_unchanged k s s' t"
 
 fun get_cl_txn :: "txid0 \<Rightarrow> cl_id" where
   "get_cl_txn (Tn_cl sn cl) = cl"
 
+fun get_sn_txn :: "txid0 \<Rightarrow> nat" where
+  "get_sn_txn (Tn_cl sn cl) = sn"
+
+fun get_txn_cl :: "cl_id \<Rightarrow> 'v global_state \<Rightarrow> txid0" where
+  "get_txn_cl cl s = Tn_cl (tm_sn (tm s cl)) cl"
+
+\<comment>\<open> Might be a good idea to check if Tn_cl sn cl = t. Not used yet.\<close>
+definition tid_match :: "'v global_state \<Rightarrow> txid0 \<Rightarrow> bool" where
+  "tid_match s t \<equiv> tm_sn (tm s (get_cl_txn t)) = get_sn_txn t "
+
+definition global_view :: "'v v_list \<Rightarrow> key_view" where
+  "global_view vl \<equiv> {0.. (length vl)}"
+
+
 definition write2 where
-  "write2 s k v s' t \<equiv> rm_status (rms s k) t = working
-                        \<and> rm_fingerpr (rms s' k) t = update_key_fp (rm_fingerpr (rms s k) t) W v
-                        \<and> rm_status (rms s' k) t = working
-                        \<and> rm_db (rms s' k) = rm_db (rms s k)
-                        \<and> tm_other_rms_unchanged k s s' t"
+  "write2 s k v s' t \<equiv>
+    km_status (kms s k) t = working
+    \<and> km_key_fp (kms s' k) t = update_key_fp (km_key_fp (kms s k) t) W v
+    \<and> km_status (kms s' k) t = working
+    \<and> km_vl (kms s' k) = km_vl (kms s k)
+    \<and> tm_other_kms_unchanged k s s' t"
 
 definition read2 where
-  "read2 s k v s' t  \<equiv> rm_status (rms s k) t = working
-                        \<and> rm_fingerpr (rms s' k) t = update_key_fp (rm_fingerpr (rms s k) t) R v
-                        \<and> rm_status (rms s' k) t = working
-                        \<and> rm_db (rms s' k) = rm_db (rms s k)
-                        \<and> tm_other_rms_unchanged k s s' t"
+  "read2 s k v s' t  \<equiv>
+    km_status (kms s k) t = working
+    \<and> km_key_fp (kms s' k) t = update_key_fp (km_key_fp (kms s k) t) R v
+    \<and> km_status (kms s' k) t = working
+    \<and> km_vl (kms s' k) = km_vl (kms s k)
+    \<and> tm_other_kms_unchanged k s s' t"
 
 definition prepare where
-  "prepare s k s' t \<equiv> tm_status (tm s (get_cl_txn t)) = tm_prepared
-                      \<and> rm_status_trans s k s' t working prepared"
+  "prepare s k s' t \<equiv>
+    tm_status (tm s (get_cl_txn t)) = tm_prepared
+    \<and> km_status_trans s k s' t working prepared"
 
 definition acquire_rd_lock where \<comment>\<open>Read Lock acquired\<close>
-  "acquire_rd_lock s k s' t \<equiv> tm_status (tm s (get_cl_txn t)) = tm_prepared
-                  \<and> rm_fingerpr (rms s k) t W = None
-                  \<and> rm_fingerpr (rms s k) t R \<noteq> None
-                  \<and> (\<forall>t'. rm_status (rms s k) t' \<in> {working, prepared, read_lock, no_lock, notokay})
-                  \<and> rm_status_trans s k s' t prepared read_lock"
+  "acquire_rd_lock s k s' t \<equiv>
+    tm_status (tm s (get_cl_txn t)) = tm_prepared
+    \<and> km_key_fp (kms s k) t W = None
+    \<and> km_key_fp (kms s k) t R \<noteq> None
+    \<and> (\<forall>t'. km_status (kms s k) t' \<in> {working, prepared, read_lock, no_lock, notokay})
+    \<and> km_status_trans s k s' t prepared read_lock"
 
 definition acquire_wr_lock where \<comment>\<open>Write Lock acquired\<close>
-  "acquire_wr_lock s k s' t \<equiv> tm_status (tm s (get_cl_txn t)) = tm_prepared
-                  \<and> rm_fingerpr (rms s k) t W \<noteq> None
-                  \<and> (\<forall>t'. rm_status (rms s k) t' \<in> {working, prepared, no_lock, notokay})
-                  \<and> rm_status_trans s k s' t prepared write_lock"
+  "acquire_wr_lock s k s' t \<equiv>
+    tm_status (tm s (get_cl_txn t)) = tm_prepared
+    \<and> km_key_fp (kms s k) t W \<noteq> None
+    \<and> (\<forall>t'. km_status (kms s k) t' \<in> {working, prepared, no_lock, notokay})
+    \<and> km_status_trans s k s' t prepared write_lock"
 
 definition acquire_no_lock where \<comment>\<open>No Lock needed\<close>
-  "acquire_no_lock s k s' t \<equiv> tm_status (tm s (get_cl_txn t)) = tm_prepared
-                            \<and> rm_fingerpr (rms s k) t W = None
-                            \<and> rm_fingerpr (rms s k) t R = None
-                            \<and> rm_status_trans s k s' t prepared no_lock"
+  "acquire_no_lock s k s' t \<equiv>
+    tm_status (tm s (get_cl_txn t)) = tm_prepared
+    \<and> km_key_fp (kms s k) t W = None
+    \<and> km_key_fp (kms s k) t R = None
+    \<and> km_status_trans s k s' t prepared no_lock"
 
 definition nok where \<comment>\<open>Lock not available\<close>
-  "nok s k s' t \<equiv> tm_status (tm s (get_cl_txn t)) = tm_prepared \<and>
-                    ((rm_fingerpr (rms s k) t R \<noteq> None \<and>
-                      (\<exists>t'. rm_status (rms s k) t' = write_lock)) \<or>
-                     (rm_fingerpr (rms s k) t W \<noteq> None \<and>
-                      (\<exists>t'. rm_status (rms s k) t' \<in> {write_lock, read_lock}))) \<and>
-                    rm_status_trans s k s' t prepared notokay"
+  "nok s k s' t \<equiv>
+    tm_status (tm s (get_cl_txn t)) = tm_prepared
+    \<and> ((km_key_fp (kms s k) t R \<noteq> None
+        \<and> (\<exists>t'. km_status (kms s k) t' = write_lock))
+       \<or> (km_key_fp (kms s k) t W \<noteq> None
+        \<and> (\<exists>t'. km_status (kms s k) t' \<in> {write_lock, read_lock})))
+    \<and> km_status_trans s k s' t prepared notokay"
 
 definition commit where
-  "commit s k s' t \<equiv> rm_status (rms s k) t \<in> {read_lock, write_lock, no_lock}
-                      \<and> tm_status (tm s (get_cl_txn t)) = tm_committed
-                      \<and> rm_db (rms s' k) =  update_kv t (rm_fingerpr (rms s k) t)
-                                                       (tm_view (tm s)) (rm_db (rms s k)) \<comment>\<open>?\<close>
-                      \<and> rm_fingerpr (rms s' k) t = Map.empty
-                      \<and> rm_status (rms s' k) t = committed
-                      \<and> tm_other_rms_unchanged rm s s' t"
+  "commit s k s' t \<equiv>
+    km_status (kms s k) t \<in> {read_lock, write_lock, no_lock}
+    \<and> tm_status (tm s (get_cl_txn t)) = tm_committed
+    \<and> km_vl (kms s' k) =
+        update_kv_key t (km_key_fp (kms s k) t) (global_view (km_vl (kms s k))) (km_vl (kms s k))
+    \<and> km_key_fp (kms s' k) t = Map.empty
+    \<and> km_status (kms s' k) t = committed
+    \<and> tm_other_kms_unchanged k s s' t"
 
 definition abort where \<comment>\<open>Locks released (aborted)\<close>
-  "abort s k s' t \<equiv> rm_status (rms s k) t \<in> {read_lock, write_lock, no_lock, notokay}
-                    \<and> tm_status (tm s (get_cl_txn t)) = tm_aborted
-                    \<and> rm_db (rms s' k) = rm_db (rms s k)
-                    \<and> rm_fingerpr (rms s' k) t = Map.empty
-                    \<and> rm_status (rms s' k) t = aborted
-                    \<and> tm_other_rms_unchanged k s s' t"
+  "abort s k s' t \<equiv>
+    km_status (kms s k) t \<in> {read_lock, write_lock, no_lock, notokay}
+    \<and> tm_status (tm s (get_cl_txn t)) = tm_aborted
+    \<and> km_vl (kms s' k) = km_vl (kms s k)
+    \<and> km_key_fp (kms s' k) t = Map.empty
+    \<and> km_status (kms s' k) t = aborted
+    \<and> tm_other_kms_unchanged k s s' t"
 
 definition user_commit where
-  "user_commit s s' cl \<equiv> tm_status (tm s cl) = tm_init
-                      \<and> tm_status (tm s' cl) = tm_prepared
-                      \<and> tm_sn (tm s' cl) = tm_sn (tm s cl)
-                      \<and> rms s' = rms s"
+  "user_commit s s' cl \<equiv>
+    tm_status (tm s cl) = tm_init
+    \<and> tm_status (tm s' cl) = tm_prepared
+    \<and> tm_sn (tm s' cl) = tm_sn (tm s cl)
+    \<and> kms s' = kms s"
 
 definition tm_commit where
-  "tm_commit s s' cl \<equiv> let t = (Tn_cl (tm_sn (tm s cl)) cl) in
-                        tm_status (tm s cl) = tm_prepared
-                    \<and> (\<forall>k. rm_status (rms s k) t \<in> {read_lock, write_lock, no_lock})
-                    \<and> tm_status (tm s' cl) = tm_committed
-                    \<and> tm_sn (tm s' cl) = tm_sn (tm s cl)
-                    \<and> rms s' = rms s"
+  "tm_commit s s' cl \<equiv>
+    tm_status (tm s cl) = tm_prepared
+    \<and> (\<forall>k. km_status (kms s k) (get_txn_cl cl s) \<in> {read_lock, write_lock, no_lock})
+    \<and> tm_status (tm s' cl) = tm_committed
+    \<and> tm_sn (tm s' cl) = tm_sn (tm s cl)
+    \<and> kms s' = kms s"
 
 definition tm_abort where
-  "tm_abort s s' cl \<equiv> let t = (Tn_cl (tm_sn (tm s cl)) cl) in
-                     (tm_status (tm s cl) = tm_prepared
-                     \<and> (\<exists>k. rm_status (rms s k) t = notokay)
-                     \<and> (\<forall>k. rm_status (rms s k) t \<in> {read_lock, write_lock, no_lock, notokay}))
-                    \<and> tm_status (tm s' cl) = tm_aborted
-                    \<and> tm_sn (tm s' cl) = tm_sn (tm s cl)
-                    \<and> rms s' = rms s"
+  "tm_abort s s' cl \<equiv>
+    (tm_status (tm s cl) = tm_prepared
+     \<and> (\<exists>k. km_status (kms s k) (get_txn_cl cl s) = notokay)
+     \<and> (\<forall>k. km_status (kms s k) (get_txn_cl cl s) \<in> {read_lock, write_lock, no_lock, notokay}))
+    \<and> tm_status (tm s' cl) = tm_aborted
+    \<and> tm_sn (tm s' cl) = tm_sn (tm s cl)
+    \<and> kms s' = kms s"
 
 definition tm_ready_c where
-  "tm_ready_c s s' cl \<equiv> let t = (Tn_cl (tm_sn (tm s cl)) cl) in
-                        tm_status (tm s cl) = tm_committed
-                      \<and> (\<forall>k. rm_status (rms s k) t = committed)
-                      \<and> tm_status (tm s' cl) = tm_init
-                      \<and> tm_sn (tm s' cl) = Suc (tm_sn (tm s cl))
-                      \<and> rms s' = rms s"
+  "tm_ready_c s s' cl \<equiv>
+    tm_status (tm s cl) = tm_committed
+    \<and> (\<forall>k. km_status (kms s k) (get_txn_cl cl s) = committed)
+    \<and> tm_status (tm s' cl) = tm_init
+    \<and> tm_sn (tm s' cl) = Suc (tm_sn (tm s cl))
+    \<and> kms s' = kms s"
 
 definition tm_ready_a where
-  "tm_ready_a s s' cl \<equiv> let t = (Tn_cl (tm_sn (tm s cl)) cl) in
-                        tm_status (tm s cl) = tm_aborted
-                      \<and> (\<forall>k. rm_status (rms s k) t = aborted)
-                      \<and> tm_status (tm s' cl) = tm_init
-                      \<and> tm_sn (tm s' cl) = Suc (tm_sn (tm s cl))
-                      \<and> rms s' = rms s"
+  "tm_ready_a s s' cl \<equiv>
+    tm_status (tm s cl) = tm_aborted
+    \<and> (\<forall>k. km_status (kms s k) (get_txn_cl cl s) = aborted)
+    \<and> tm_status (tm s' cl) = tm_init
+    \<and> tm_sn (tm s' cl) = Suc (tm_sn (tm s cl))
+    \<and> kms s' = kms s"
 
-consts cl0 :: cl_id
 text\<open>The Event System\<close>
 definition gs_init :: "'v global_state" where
   "gs_init \<equiv> \<lparr> 
     tm = (\<lambda>cl. \<lparr> tm_status = tm_init, tm_sn = 0 \<rparr>),
-    rms = (\<lambda>k. \<lparr> rm_db = [version_init],
-                 rm_fingerpr = (\<lambda>t. Map.empty), 
-                 rm_status = (\<lambda>t. working)\<rparr>)
+    kms = (\<lambda>k. \<lparr> km_vl = [version_init],
+                 km_key_fp = (\<lambda>t. Map.empty), 
+                 km_status = (\<lambda>t. working)\<rparr>)
   \<rparr>"
 
 fun gs_trans :: "'v global_state \<Rightarrow> 'v ev \<Rightarrow> 'v global_state \<Rightarrow> bool" where
-  "gs_trans s (RM_ev k (Write2 t v)) s' \<longleftrightarrow> write2 s k v s' t" |
-  "gs_trans s (RM_ev k (Read2 t v))  s' \<longleftrightarrow> read2 s k v s' t" |
-  "gs_trans s (RM_ev k (Prepare t))  s' \<longleftrightarrow> prepare s k s' t" |
-  "gs_trans s (RM_ev k (RLock t))    s' \<longleftrightarrow> acquire_rd_lock s k s' t" |
-  "gs_trans s (RM_ev k (WLock t))    s' \<longleftrightarrow> acquire_wr_lock s k s' t" |
-  "gs_trans s (RM_ev k (NoLock t))   s' \<longleftrightarrow> acquire_no_lock s k s' t" |
-  "gs_trans s (RM_ev k (NOK t))      s' \<longleftrightarrow> nok s k s' t" |
-  (*"gs_trans s (RM_ev k (Commit t))   s' \<longleftrightarrow> commit s k s'" |*)
-  "gs_trans s (RM_ev k (Abort t))    s' \<longleftrightarrow> abort s k s' t" |
+  "gs_trans s (KM_ev k (Write2 t v)) s' \<longleftrightarrow> write2 s k v s' t" |
+  "gs_trans s (KM_ev k (Read2 t v))  s' \<longleftrightarrow> read2 s k v s' t" |
+  "gs_trans s (KM_ev k (Prepare t))  s' \<longleftrightarrow> prepare s k s' t" |
+  "gs_trans s (KM_ev k (RLock t))    s' \<longleftrightarrow> acquire_rd_lock s k s' t" |
+  "gs_trans s (KM_ev k (WLock t))    s' \<longleftrightarrow> acquire_wr_lock s k s' t" |
+  "gs_trans s (KM_ev k (NoLock t))   s' \<longleftrightarrow> acquire_no_lock s k s' t" |
+  "gs_trans s (KM_ev k (NOK t))      s' \<longleftrightarrow> nok s k s' t" |
+  "gs_trans s (KM_ev k (Commit t))   s' \<longleftrightarrow> commit s k s' t" |
+  "gs_trans s (KM_ev k (Abort t))    s' \<longleftrightarrow> abort s k s' t" |
   "gs_trans s (TM_ev cl User_Commit) s' \<longleftrightarrow> user_commit s s' cl" |
   "gs_trans s (TM_ev cl TM_Commit)   s' \<longleftrightarrow> tm_commit s s' cl" |
   "gs_trans s (TM_ev cl TM_Abort)    s' \<longleftrightarrow> tm_abort s s' cl" |
@@ -191,7 +217,7 @@ definition tps :: "('v ev, 'v global_state) ES" where
   \<rparr>"
 
 lemmas tps_trans_defs = write2_def read2_def prepare_def acquire_rd_lock_def acquire_wr_lock_def
-                        acquire_no_lock_def nok_def (*commit_def*) abort_def
+                        acquire_no_lock_def nok_def commit_def abort_def
                         user_commit_def tm_commit_def tm_abort_def tm_ready_c_def tm_ready_a_def
 
 lemmas tps_defs = tps_def gs_init_def
